[minor] encoding for cfi tags

cfi/main.v
@@ -1,8 +1,8 @@
-Require Import ssreflect ssrbool eqtype.
+Require Import ssreflect ssrbool ssrfun eqtype.
 
-Require Import lib.Coqlib.
-Require Import lib.utils.
-Require Import lib.partial_maps.
+Require Import Coq.Lists.List. 
+Require Import lib.Coqlib lib.utils.
+Require Import lib.partial_maps lib.FiniteMaps lib.ordered.
 Require Import common.common.
 Require Import concrete.concrete.
 Require Import concrete.int_32.
@@ -16,15 +16,208 @@ Require Import cfi.rules.
 Require Import cfi.symbolic.
 Require Import cfi.abstract.
 Require Import cfi.refinementAS.
+Require Import Integers.
+
+Module NatPMap := FiniteMap NatIndexed.
+
+Instance nat_partial_map : PartMaps.partial_map NatPMap.t nat := {
+  get V m n := NatPMap.get n m;
+  set V m n v := NatPMap.set n v m;
+  map_filter V1 V2 f m := NatPMap.map_filter f m;
+  empty V := NatPMap.empty _
+}.
+
+Instance nat_partial_map_axioms : PartMaps.axioms nat_partial_map.
+Proof.
+  constructor.
+  - (* get_set_eq *) intros V m n v. by apply NatPMap.gss.
+  - (* get_set_neq *) intros V m n1 n2 v. by apply NatPMap.gso.
+  - (* map_filter_correctness *) intros V1 V2 f m k. by apply NatPMap.gmap_filter.
+  - (* empty_is_empty *) intros V k. by apply NatPMap.gempty.
+Qed.
+
+Module CFIInstances.
+
+Section WithClasses.
+
+(* ---------------------------------------------------------------- *)
+(* int32 instance *)
+
+Definition t := concrete_int_32_t.
+Instance ops : machine_ops t := concrete_int_32_ops.
+
+Definition id_size := Word.int 27.
+Definition id := [eqType of id_size].
+Definition bound : word t := Word.repr ((Word.max_unsigned 27) + 1)%Z. (*29 bits*)
+
+Definition word_to_id (w : word t) : option id_size :=
+  if (Word.ltu w bound) then Some (Word.castu w) else None.
+
+Definition id_to_word (x : id) : word t := 
+  Word.castu x.
+
+Lemma id_to_word_bound x : Word.ltu (id_to_word x) bound.
+Proof.
+  destruct x as [x Hx]. 
+  let u := eval compute in (Word.modulus 27) in
+  change (Word.modulus 27) with u in Hx.
+  unfold id_to_word, Word.castu, Word.ltu, bound.
+  simpl. rewrite Word.Z_mod_modulus_eq. rewrite Zmod_small. 
+  - destruct (zlt x 268435456); by [trivial | omega].
+  -  let u := eval compute in (Word.modulus 31) in
+     change (Word.modulus 31) with u.
+     by omega.
+Qed.
+  
+Lemma id_to_wordK x : word_to_id (id_to_word x) = Some x.
+Proof.
+  remember (id_to_word x) as w eqn:Hw.
+  unfold word_to_id.
+  rewrite Hw. clear Hw.
+  rewrite id_to_word_bound.
+  unfold id_to_word, Word.castu, bound in *.
+  apply f_equal.
+  rewrite Word.unsigned_repr_eq.
+  let u := eval compute in (Word.modulus (word_size_minus_one t)) in
+  change (Word.modulus (word_size_minus_one t)) with u.
+  rewrite Zmod_small.
+  - by apply Word.repr_unsigned.
+  - unfold Word.unsigned. 
+    assert (H := Word.intrange 27 x).
+    let u := eval compute in (Word.modulus 27) in
+                              change (Word.modulus 27) with u in H.
+    by omega.
+Qed.
+
+Lemma word_to_idK w x :
+  word_to_id w = Some x ->
+  id_to_word x = w.
+Proof.
+  intros Hwid.
+  unfold word_to_id in Hwid.
+  destruct (Word.ltu w bound) eqn:Hl; [idtac | discriminate].
+  inv Hwid.
+  unfold id_to_word, Word.castu.
+  rewrite Word.unsigned_repr_eq.
+  let u := eval compute in (Word.modulus 27) in
+                            change (Word.modulus 27) with u.
+  unfold Word.ltu, bound in Hl.
+  simpl in Hl.
+  case: (zlt (Word.unsigned w) 268435456) => Hcmp.
+  + rewrite Zmod_small; [by apply Word.repr_unsigned | idtac].
+    split; auto. 
+    destruct (Word.unsigned_range w) as [? ?].
+    by assumption.
+  + exfalso. 
+    apply zlt_false with (A := bool) (a := true) (b := false) in Hcmp.
+    rewrite Hl in Hcmp.
+    by discriminate.
+Qed.
+    
+Instance ids : cfi_id := {|
+ id := id;
+ word_to_id := word_to_id;
+ id_to_word := id_to_word
+|}.
+Proof.
+  - by apply id_to_wordK.
+  - by apply word_to_idK.
+Defined.
+
+(* Encoding of tags:
+      DATA           --> 0
+      INSTR None     --> 1
+      INSTR (Some x) --> x*4+2
+*)
+
+Import Word.Notations List.ListNotations.
+
+Definition encode_cfi_tag (t : cfi_tag) : Word.int 29 :=
+ match t with
+   DATA => Word.pack [27; 1] [Word.zero; Word.zero]%wp
+ | INSTR None => Word.pack [27; 1] [Word.zero; Word.one]%wp
+ | INSTR (Some x) => Word.pack [27; 1] [x; Word.repr 2]%wp
+ end.
+
+Definition decode_cfi_tag (t : Word.int 29) : option cfi_tag :=
+  let: [k; t]%wu := Word.unpack [27; 1] t in
+  if t == Word.zero then
+    if k == Word.zero then Some DATA
+    else None
+  else if t == Word.one then
+    if k == Word.zero then Some (INSTR None)
+    else None
+  else if t == Word.repr 2 then
+    Some (INSTR (Some k))
+  else None.
+
+Lemma encode_cfi_tagK t : decode_cfi_tag (encode_cfi_tag t) = Some t.
+Proof.
+  case: t => [[k|]|];
+  by rewrite /decode_cfi_tag /encode_cfi_tag Word.packK /=.
+Qed.
+
+Lemma decode_cfi_tagK w t : decode_cfi_tag w = Some t ->
+                                encode_cfi_tag t = w.
+Proof.
+  rewrite /decode_cfi_tag /encode_cfi_tag.
+  case E: (Word.unpack [27; 1] w) => [k [w' []]].
+  move: (Word.unpackK [27; 1] w). rewrite E.
+  have [?|?] := altP (w' =P Word.zero); try subst w'.
+  { have [?|?] := altP (k =P Word.zero); try subst k; last by [].
+    by move => H [<-]. }
+  have [?|?] := altP (w' =P Word.one); try subst w'.
+  { have [?|?] := altP (k =P Word.zero); try subst k; last by [].
+     by move => H [<-]. }
+  have [?|?] := altP (w' =P Word.repr 2); try subst w'; last by [].
+  by move => H [<-].
+Qed.
+
+Import DoNotation.
+
+Instance encodable_tag : @encodable cfi_tag_eqType t := {|
+  encode t :=
+    match t with
+    | USER ut => Word.pack [29; 1] [encode_cfi_tag ut; Word.one]%wp
+    | ENTRY ut => Word.pack [29; 1] [encode_cfi_tag ut; Word.repr 2]%wp
+    | KERNEL => Word.pack [29; 1] [Word.zero; Word.zero]%wp
+    end;
+
+  decode w :=
+    let: [ut; w']%wu := Word.unpack [29; 1] w in
+    if w' == Word.zero then
+      if ut == Word.zero then Some KERNEL
+      else None
+    else if w' == Word.one then
+      do! ut <- decode_cfi_tag ut;
+      Some (@USER cfi_tag_eqType ut)
+    else if w' == Word.repr 2 then
+      do! ut <- decode_cfi_tag ut;
+      Some (@ENTRY cfi_tag_eqType ut)
+    else None;
+
+  encode_kernel_tag := erefl
+|}.
+Proof.
+  - case => [ut| |ut];
+    by rewrite Word.packK /= ?encode_cfi_tagK.
+  - intros t w.
+    case E: (Word.unpack [29; 1] w) => [ut [w' []]].
+    move: (Word.unpackK [29; 1] w). rewrite E.
+    have [?|?] := altP (w' =P Word.zero); try subst w'.
+    { have [?|?] := altP (ut =P Word.zero); try subst ut; last by [].
+      by move => H [<-]. }
+    have [?|?] := altP (w' =P Word.one); try subst w'.
+    { case DEC: (decode_cfi_tag ut) => [ut'|] //=.
+      apply decode_cfi_tagK in DEC. subst ut.
+      by move => H [<-]. }
+    have [?|?] := altP (w' =P Word.repr 2); try subst w'; last by [].
+    case DEC: (decode_cfi_tag ut) => [ut'|] //=.
+    apply decode_cfi_tagK in DEC. subst ut.
+    by move => H [<-].
+Qed.
 
 Section Refinement.
-
-Let t := concrete_int_32_t.
-Existing Instance concrete_int_32_ops.
-Existing Instance concrete_int_32_ops_spec.
-
-Context {ids : @classes.cfi_id t}
-        {enc : @rules.encodable rules.cfi_tag_eqType t}.
 
 Variable cfg : id -> id -> bool.
 
@@ -102,4 +295,10 @@ Proof.
   intros (ast' & EXECA & AS'). eauto 7.
 Qed.
 
+
+
 End Refinement.
+
+End WithClasses.
+
+End CFIInstances.
